$$
d(X,X') = \sqrt{ \sum_i \sum_\alpha^{x,y,z}  \frac{w_i}{\sum_j w_j} ( X _{i,\alpha}-com _\alpha(X)-{X'} _{i,\alpha}+com _\alpha(X') )^2 }
$$

with

$$
com_\alpha (X) = \sum_i \frac{w'_{i}}{\sum_j w'_j} X _{i,\alpha}
$$

and

$$
com_\alpha(X')= \sum_i  \frac{w'_{i}}{\sum_j w'_j}X' _{i,\alpha}
$$

$$
\begin{align}
X & = \frac{\sum_i X_i*\exp(-\lambda D_i(x))}{\sum_i  \exp(-\lambda D_i(x))} \\
Y & = \frac{\sum_i Y_i*\exp(-\lambda D_i(x))}{\sum_i  \exp(-\lambda D_i(x))} \\
& \cdots\\
zzz & =-\frac{1}{\lambda}\log(\sum_i  \exp(-\lambda D_i(x)))
\end{align}
$$ 

$$
\AA
$$


